PREFIX altr: <http://www.w3.org/ns/dx/connegp/altr#>
PREFIX dcterms: <http://purl.org/dc/terms/>
PREFIX owl: <http://www.w3.org/2002/07/owl#>
PREFIX rdf: <http://www.w3.org/1999/02/22-rdf-syntax-ns#>
PREFIX sdo: <https://schema.org/>
PREFIX xsd: <http://www.w3.org/2001/XMLSchema#>
PREFIX rdfs: <http://www.w3.org/2000/01/rdf-schema#>
PREFIX skos: <http://www.w3.org/2004/02/skos/core#>

<http://www.w3.org/ns/dx/connegp/altr>
    a owl:Ontology ;
    rdfs:label "Alternative Profiles Ontology" ;
    rdfs:comment """This ontology allows for the description of representations of Internet resources.

Representations may conform to prof:Profile instances and may have the format of a particular dcterms:MediaType."""@en ;
    dcterms:created "2019-08-07"^^xsd:date ;
    dcterms:modified "2024-02-07"^^xsd:date ;
    dcterms:creator [
        a sdo:Person ;
        sdo:affiliation <https://kurrawong.ai> ;
        sdo:email <mailto:nick@kurrawong.ai> ;
        sdo:identifier <http://orcid.org/0000-0002-8742-7730> ;
        sdo:name "Nicholas J. Car" ;
    ] ;
.

<https://kurrawong.ai>
    a sdo:Organization ;
    sdo:name "KurrawongAI" ;
    sdo:url "https://kurrawong.ai"^^xsd:anyURI ;
.

dcterms:conformsTo
    a owl:ObjectProperty ;
    rdfs:label "conforms to" ;
    dcterms:source dcterms:conformsTo ;
    skos:scopeNote "In the context of the Alternative Profiles Ontology, use this property to indicate a dcterms:Standard that a altr:Representation conforms to." ;
.

altr:hasRepresentation
    a owl:ObjectProperty ;
    rdfs:label "has representation" ;
    skos:definition "Indicates a Representation of a Resource."@en ;
    rdfs:domain rdfs:Resource ;
    rdfs:range altr:Representation ;
    skos:scopeNote "Use this property to indicate an HTTP-delivered representation of a resource." ;
.

altr:hasDefaultRepresentation
    a owl:ObjectProperty ;
    rdfs:label "has default representation" ;
    skos:definition "Indicates the default Representation of a Resource."@en ;
    rdfs:domain altr:Representation ;
    rdfs:subPropertyOf altr:hasRepresentation ;
    skos:scopeNote "Use this property to indicate the default HTTP-delivered representation of a resource that is obtained when no further instructions are given to a server to obtain a resource's representation other than the identification (URI) of the resource" ;
.

rdfs:Resource
    a owl:Class ;
    rdfs:label "Resource" ;
    skos:definition "The class resource, everything."@en ;
    dcterms:source "http://www.w3.org/2000/01/rdf-schema#Resource" ;
    skos:scopeNote "In the context of the Alternative Profiles Ontology, rdfs:Resource instances are used to identify Internet resources, that is items identified by a URI." ;
.

altr:Representation
    a owl:Class ;
    rdfs:label "Representation" ;
    skos:definition "An abstraction of the current or desired state of a thing in HTTP communications."@en ;
    dcterms:source <https://httpwg.org/specs/rfc7230.html> ;
    rdfs:isDefinedBy <http://www.w3.org/ns/dx/connegp/altr> ;
    skos:scopeNote "Use this class to indicate instances of representations of resources" ;
.

dcterms:Standard
    a owl:Class ;
    rdfs:label "Standard" ;
    skos:definition "A basis for comparison; a reference point against which other things can be evaluated."@en ;
    dcterms:source "http://purl.org/dc/terms/Standard" ;
    skos:scopeNote "In the context of the Alternative Profiles Ontology, use this class to indicate instances of information models that representations of resources can conform to." ;
.
